examples/nothing.v
@@ -26,45 +26,48 @@ Module Nothing.
 
   (* Typechecking  *)
   Definition rules :=
-    tc_rules R empty_Sigma
-             (fun r => match r with
-                    | tick => _tick
-                    end).
+    tc_rules R empty_Sigma (fun r => match r with tick => _tick end).
 
   Definition cycle_log :=
     tc_compute (interp_scheduler cr empty_sigma rules nothing).
 
   Definition tick_result :=
-    tc_compute (interp_action cr empty_sigma CtxEmpty log_empty log_empty
-                              (rules tick)).
+    tc_compute (
+      interp_action cr empty_sigma CtxEmpty log_empty log_empty (rules tick)
+    ).
 
-  Definition result :=
-    tc_compute (commit_update cr cycle_log).
+  Definition result := tc_compute (commit_update cr cycle_log).
 
   Definition external (r: rule_name_t) := false.
 
-  Definition circuits :=
-    compile_scheduler rules external nothing.
-
+  Definition circuits := compile_scheduler rules external nothing.
   Definition circuits_result :=
-    tc_compute (interp_circuits empty_sigma circuits (lower_r (ContextEnv.(create) r))).
+    tc_compute (
+      interp_circuits empty_sigma circuits (lower_r (ContextEnv.(create) r))
+    ).
 
-  Example test: circuits_result = Environments.map _ (fun _ => bits_of_value) result :=
-    eq_refl.
+  Example test:
+    circuits_result = Environments.map _ (fun _ => bits_of_value) result
+  := eq_refl.
 
-  Definition package :=
-    {| ip_koika := {| koika_reg_types := R;
-                     koika_reg_init := r;
-                     koika_ext_fn_types := empty_Sigma;
-                     koika_rules := rules;
-                     koika_rule_external := external;
-                     koika_scheduler := nothing;
-                     koika_module_name := "nothing" |};
-
-       ip_sim := {| sp_ext_fn_specs := empty_ext_fn_props;
-                   sp_prelude := None |};
-
-       ip_verilog := {| vp_ext_fn_specs := empty_ext_fn_props |} |}.
+  Definition package := {|
+    ip_koika := {|
+      koika_reg_types := R;
+      koika_reg_init := r;
+      koika_ext_fn_types := empty_Sigma;
+      koika_rules := rules;
+      koika_rule_external := external;
+      koika_scheduler := nothing;
+      koika_module_name := "nothing"
+    |};
+    ip_sim := {|
+      sp_ext_fn_specs := empty_ext_fn_props;
+      sp_prelude := None
+    |};
+    ip_verilog := {|
+      vp_ext_fn_specs := empty_ext_fn_props
+    |}
+  |}.
 End Nothing.
 
 Definition prog := Interop.Backends.register Nothing.package.
